-

AbGroup.v
@@ -92,3 +92,342 @@ Arguments H_app [A] [B].
 Arguments H_mem_compat _ _ f : rename.
 Arguments H_app_compat _ _ f : rename.
 Arguments H_additive _ _ f : rename.
+
+(* Equality (gr_eq) in groups is an equivalence relation *)
+
+Add Parametric Relation {G} : (gr_set G) (@gr_eq G)
+ reflexivity proved by (@Equivalence_Reflexive _ (@gr_eq G) (@gr_equiv G))
+ symmetry proved by (@Equivalence_Symmetric _ (@gr_eq G) (@gr_equiv G))
+ transitivity proved by (@Equivalence_Transitive _ (@gr_eq G) (@gr_equiv G))
+ as gr_eq_rel.
+
+(* Coq "Morphisms": they allow to use "rewrite" in expressions containing
+   inversions (-), additions (+) and memberships (∈) *)
+
+Add Parametric Morphism {G} : (@gr_inv G)
+  with signature @gr_eq G ==> @gr_eq G
+  as gr_inv_morph.
+Proof.
+intros * Hxy.
+now apply gr_inv_compat.
+Qed.
+
+Add Parametric Morphism {G} : (@gr_add G)
+  with signature @gr_eq G ==> @gr_eq G ==> @gr_eq G
+  as gr_add_morph.
+Proof.
+intros * Hxy x' y' Hxy'.
+now apply gr_add_compat.
+Qed.
+
+Add Parametric Morphism {G} : (@gr_mem G)
+  with signature @gr_eq G ==> iff
+  as gr_mem_morph.
+Proof.
+intros * Hxy.
+split; intros H.
+-eapply gr_mem_compat; [ apply Hxy | easy ].
+-eapply gr_mem_compat; [ symmetry; apply Hxy | easy ].
+Qed.
+
+(*
+Definition gr_elem A := { a : gr_set A | a ∈ A }.
+Definition gr_mem_eq A (x y : gr_elem A) := (proj1_sig x = proj1_sig y)%G.
+
+Theorem gr_mem_refl {A} : Reflexive (gr_mem_eq A).
+Proof.
+intros (x & Hx).
+now unfold gr_mem_eq.
+Qed.
+
+Theorem gr_mem_symm {A} : Symmetric (gr_mem_eq A).
+Proof.
+intros (x & Hx) (y & Hy).
+unfold gr_mem_eq; simpl; intros Hxy.
+now symmetry.
+Qed.
+
+Theorem gr_mem_trans {A} : Transitive (gr_mem_eq A).
+Proof.
+intros (x & Hx) (y & Hy) (z & Hz).
+unfold gr_mem_eq; simpl; intros Hxy Hyz.
+now transitivity y.
+Qed.
+
+Add Parametric Relation {G} : _ (@gr_mem_eq G)
+ reflexivity proved by gr_mem_refl
+ symmetry proved by gr_mem_symm
+ transitivity proved by gr_mem_trans
+ as gr_mem_rel.
+
+Definition M_app A B (f : HomGr A B) (x : gr_elem A) := H_app f (proj1_sig x).
+
+Add Parametric Morphism {G H} : (M_app G H)
+  with signature eq ==> gr_mem_eq G ==> @gr_eq H
+  as M_app_morph.
+Proof.
+intros f (x, Hx) (y, Hy) Hxy.
+unfold gr_mem_eq in Hxy; simpl in Hxy.
+unfold M_app; simpl.
+now apply H_app_compat.
+Qed.
+*)
+
+(* Miscellaneous theorems in groups *)
+
+Theorem gr_add_0_r : ∀ G (x : gr_set G), (x + 0 = x)%G.
+Proof.
+intros.
+rewrite gr_add_comm.
+apply gr_add_0_l.
+Qed.
+
+Theorem gr_add_inv_l : ∀ G (x : gr_set G), (- x + x = 0)%G.
+Proof.
+intros.
+rewrite gr_add_comm.
+apply gr_add_inv_r.
+Qed.
+
+Theorem gr_inv_zero : ∀ G, (- 0 = @gr_zero G)%G.
+Proof.
+intros.
+rewrite <- gr_add_0_l.
+apply gr_add_inv_r.
+Qed.
+
+Theorem gr_sub_0_r : ∀ G (x : gr_set G), (x - 0 = x)%G.
+Proof.
+intros.
+symmetry; rewrite <- gr_add_0_r at 1.
+apply gr_add_compat; [ easy | now rewrite gr_inv_zero ].
+Qed.
+
+Theorem gr_sub_move_r : ∀ G (x y z : gr_set G),
+  (x - y = z)%G ↔ (x = z + y)%G.
+Proof.
+intros.
+split; intros Hxyz.
+-now rewrite <- Hxyz, gr_add_assoc, gr_add_inv_l, gr_add_0_r.
+-now rewrite Hxyz, gr_add_assoc, gr_add_inv_r, gr_add_0_r.
+Qed.
+
+Theorem gr_sub_move_l : ∀ G (x y z : gr_set G),
+  (x - y = z)%G ↔ (x = y + z)%G.
+Proof.
+intros.
+split; intros Hxyz.
+-now rewrite <- Hxyz, gr_add_comm, gr_add_assoc, gr_add_inv_l, gr_add_0_r.
+-now rewrite Hxyz, gr_add_comm, <- gr_add_assoc, gr_add_inv_l, gr_add_0_l.
+Qed.
+
+Theorem gr_inv_add_distr : ∀ G (x y : gr_set G), (- (x + y) = - x - y)%G.
+Proof.
+intros *.
+symmetry.
+apply gr_sub_move_r.
+rewrite <- gr_add_0_l.
+apply gr_sub_move_r.
+symmetry; rewrite gr_add_assoc.
+symmetry.
+apply gr_sub_move_r.
+rewrite gr_add_0_l.
+apply gr_inv_compat, gr_add_comm.
+Qed.
+
+Theorem gr_inv_involutive : ∀ G (x : gr_set G), (- - x = x)%G.
+Proof.
+intros.
+transitivity (- - x + (- x + x))%G.
+-rewrite <- gr_add_0_r at 1.
+ apply gr_add_compat; [ easy | ].
+ now rewrite gr_add_inv_l.
+-now rewrite <- gr_add_assoc, gr_add_inv_l, gr_add_0_l.
+Qed.
+
+Theorem gr_eq_inv_l : ∀ G (x y : gr_set G), (- x = y)%G ↔ (x = - y)%G.
+Proof.
+intros.
+split; intros Hxy.
+-rewrite <- Hxy; symmetry; apply gr_inv_involutive.
+-rewrite Hxy; apply gr_inv_involutive.
+Qed.
+
+(* Theorems on homomorphisms *)
+
+Theorem H_zero : ∀ A B (f : HomGr A B), (H_app f 0 = 0)%G.
+Proof.
+intros.
+assert (H1 : (@gr_zero A + 0 = 0)%G) by apply A.
+assert (H2 : (H_app f 0 + H_app f 0 = H_app f 0)%G). {
+  rewrite <- H_additive; [ | apply A | apply A ].
+  apply f; [ apply A; apply A | apply A | easy ].
+}
+assert (H3 : (H_app f 0 + H_app f 0 - H_app f 0 = H_app f 0 - H_app f 0)%G). {
+  apply gr_add_compat; [ apply H2 | easy ].
+}
+assert (H4 : (H_app f 0 + H_app f 0 - H_app f 0 = 0)%G). {
+  rewrite H3; apply gr_add_inv_r.
+}
+rewrite <- H4.
+now rewrite gr_add_assoc, gr_add_inv_r, gr_add_0_r.
+Qed.
+
+Theorem H_inv : ∀ A B (f : HomGr A B) x,
+  x ∈ A → (H_app f (- x) = - H_app f x)%G.
+Proof.
+intros * Hx.
+assert (H1 : (x - x = 0)%G) by apply A.
+assert (H2 : (H_app f (x - x) = H_app f 0)%G). {
+  apply H_app_compat; [ now apply A, A | apply A | apply H1 ].
+}
+assert (H3 : (H_app f x + H_app f (- x) = H_app f 0)%G). {
+  rewrite <- H2.
+  symmetry; apply H_additive; [ easy | now apply A ].
+}
+assert (H4 : (H_app f x + H_app f (- x) = 0)%G). {
+  rewrite H3; apply H_zero.
+}
+symmetry; rewrite <- gr_add_0_l.
+apply gr_sub_move_l.
+now symmetry.
+Qed.
+
+(* Images *)
+
+Theorem Im_zero_mem {G H} : ∀ (f : HomGr G H),
+  ∃ a : gr_set G, a ∈ G ∧ (H_app f a = 0)%G.
+Proof.
+intros.
+exists 0%G.
+split; [ apply gr_zero_mem | apply H_zero ].
+Qed.
+
+Theorem Im_add_mem {G H} : ∀ f (x y : gr_set H),
+  (∃ a : gr_set G, a ∈ G ∧ (H_app f a = x)%G)
+  → (∃ a : gr_set G, a ∈ G ∧ (H_app f a = y)%G)
+  → ∃ a : gr_set G, a ∈ G ∧ (H_app f a = x + y)%G.
+Proof.
+intros f y y' (x & Hxg & Hx) (x' & Hx'g & Hx').
+exists (gr_add x x').
+split; [ now apply G | ].
+rewrite H_additive; [ | easy | easy ].
+now apply gr_add_compat.
+Qed.
+
+Theorem Im_inv_mem {G H} : ∀ (f : HomGr G H) (x : gr_set H),
+  (∃ a : gr_set G, a ∈ G ∧ (H_app f a = x)%G)
+  → ∃ a : gr_set G, a ∈ G ∧ (H_app f a = - x)%G.
+Proof.
+intros f x (y & Hy & Hyx).
+exists (gr_inv y).
+split; [ now apply gr_inv_mem | ].
+rewrite <- Hyx.
+now apply H_inv.
+Qed.
+
+Theorem Im_mem_compat {G H} : ∀ f (x y : gr_set H),
+  (x = y)%G
+  → (∃ a, a ∈ G ∧ (H_app f a = x)%G)
+  → ∃ a, a ∈ G ∧ (H_app f a = y)%G.
+intros * Hxy (z & Hz & Hfz).
+exists z.
+split; [ easy | now rewrite Hfz ].
+Qed.
+
+Definition Im {G H : AbGroup} (f : HomGr G H) :=
+  {| gr_set := gr_set H;
+     gr_zero := gr_zero;
+     gr_eq := @gr_eq H;
+     gr_mem := λ b, ∃ a, a ∈ G ∧ (H_app f a = b)%G;
+     gr_add := @gr_add H;
+     gr_inv := @gr_inv H;
+     gr_zero_mem := Im_zero_mem f;
+     gr_add_mem := Im_add_mem f;
+     gr_add_0_l := gr_add_0_l H;
+     gr_add_assoc := gr_add_assoc H;
+     gr_inv_mem := Im_inv_mem f;
+     gr_add_inv_r := gr_add_inv_r H;
+     gr_add_comm := gr_add_comm H;
+     gr_equiv := gr_equiv H;
+     gr_mem_compat := Im_mem_compat f;
+     gr_add_compat := gr_add_compat H;
+     gr_inv_compat := gr_inv_compat H |}.
+
+(* Kernels *)
+
+Theorem Ker_zero_mem {G H} : ∀ (f : HomGr G H), 0%G ∈ G ∧ (H_app f 0 = 0)%G.
+Proof.
+intros f.
+split; [ apply gr_zero_mem | apply H_zero ].
+Qed.
+
+Theorem Ker_add_mem {G H} : ∀ (f : HomGr G H) (x y : gr_set G),
+  x ∈ G ∧ (H_app f x = 0)%G
+  → y ∈ G ∧ (H_app f y = 0)%G → (x + y)%G ∈ G ∧ (H_app f (x + y) = 0)%G.
+Proof.
+intros f x x' (Hx, Hfx) (Hx', Hfx').
+split; [ now apply gr_add_mem | ].
+rewrite H_additive; [ | easy | easy ].
+rewrite Hfx, Hfx'.
+apply gr_add_0_r.
+Qed.
+
+Theorem Ker_inv_mem {G H} : ∀ (f : HomGr G H) (x : gr_set G),
+  x ∈ G ∧ (H_app f x = 0)%G → (- x)%G ∈ G ∧ (H_app f (- x) = 0)%G.
+Proof.
+intros f x (Hx & Hfx).
+split; [ now apply gr_inv_mem | ].
+rewrite H_inv; [ | easy ].
+rewrite Hfx.
+apply gr_inv_zero.
+Qed.
+
+Theorem Ker_mem_compat {G H} : ∀ (f : HomGr G H) x y,
+  (x = y)%G → x ∈ G ∧ (H_app f x = 0)%G → y ∈ G ∧ (H_app f y = 0)%G.
+Proof.
+intros * Hxy (ax, Hx).
+split.
+-eapply gr_mem_compat; [ apply Hxy | easy ].
+-rewrite <- Hx.
+ apply f; [ | easy | easy ].
+ now rewrite <- Hxy.
+Qed.
+
+Definition Ker {G H : AbGroup} (f : HomGr G H) :=
+  {| gr_set := gr_set G;
+     gr_zero := gr_zero;
+     gr_eq := @gr_eq G;
+     gr_mem := λ a, a ∈ G ∧ (H_app f a = gr_zero)%G;
+     gr_add := @gr_add G;
+     gr_inv := @gr_inv G;
+     gr_zero_mem := Ker_zero_mem f;
+     gr_add_mem := Ker_add_mem f;
+     gr_add_0_l := gr_add_0_l G;
+     gr_add_assoc := gr_add_assoc G;
+     gr_inv_mem := Ker_inv_mem f;
+     gr_add_inv_r := gr_add_inv_r G;
+     gr_add_comm := gr_add_comm G;
+     gr_equiv := gr_equiv G;
+     gr_mem_compat := Ker_mem_compat f;
+     gr_add_compat := gr_add_compat G;
+     gr_inv_compat := gr_inv_compat G |}.
+
+(* Exact sequences *)
+
+Inductive sequence {A : AbGroup} :=
+  | SeqEnd : sequence
+  | Seq : ∀ {B} (f : HomGr A B), @sequence B → sequence.
+
+Notation "A ⊂ B" := (∀ a, a ∈ A → a ∈ B) (at level 60).
+Notation "A == B" := (A ⊂ B ∧ B ⊂ A) (at level 60).
+
+Fixpoint exact_sequence {A : AbGroup} (S : sequence) :=
+  match S with
+  | SeqEnd => True
+  | Seq f S' =>
+      match S' with
+      | SeqEnd => True
+      | Seq g S'' => Im f == Ker g ∧ exact_sequence S'
+      end
+  end.
